Add Twitter

examples/Twitter/Twitter-Instrumented-PC.bpl
@@ -1,40 +1,41 @@
 // Twitter Application
+// It has 3 transactions: register, fellowUser, and addTweet
+// Non-robustness check between CC and PC
+// RUN: /usr/bin/time -v --format="%e" %boogie -noinfer -typeEncoding:m -tracePOs -traceTimes  -trace  -useArrayTheory "%s" > "%t"
+// RUN: %diff "%s.expect" "%t"
 
 type Pid;
 type Uid;
 
 function {:builtin "MapConst"} MapConstBool(bool) : [Pid]bool;
-function {:inline} {:linear "pid"} TidCollector(x: Pid) : [Pid]bool
+function {:inline} {:linear "pid"} PidCollector(x: Pid) : [Pid]bool
 {
   MapConstBool(false)[x := true]
 }
 
 function {:builtin "MapConst"} MapConstBool2(bool) : [Uid]bool;
-function {:inline} {:linear "uid"} TidCollector2(x: Uid) : [Uid]bool
+function {:inline} {:linear "uid"} UidCollector(x: Uid) : [Uid]bool
 {
   MapConstBool2(false)[x := true]
 }
 
-var {:layer 0,2} ActiveUser: [Uid]bool;
+var {:layer 0,2} RegistredUsers: [Uid]bool;
 var {:layer 0,2} UserPassword: [Uid]int;
 var {:layer 0,2} UserFollow: [Uid][Uid]bool;
 var {:layer 0,2} UserTweetFollowers: [Uid][Uid]int;
 
-// secondary shared variables to simulate disabled writes and reads
+//////////////////////////////////////////////
+// Auxiliary variables for the instrumentation:
+//////////////////////////////////////////////
 
 var {:layer 0,2} copyUserFollow: [Uid][Uid]bool;
 var {:layer 0,2} copyUserTweetFollowers: [Uid][Uid]int;
 
-
-
-// 
 var {:layer 0,2} hb : bool;
-
 
 var {:layer 0,2} att : bool;
 
 var {:layer 0,2} hbd: [Pid][Uid][Uid]int; // to track dependency access to the table UserFollow
-
 
 var {:layer 0,2} varAtt1 : Uid;
 var {:layer 0,2} varAtt2 : Uid;
@@ -42,7 +43,6 @@ var {:layer 0,2} varAtt2 : Uid;
 const unique lda, sta: int;
 
 axiom ((lda == 1) && (sta == 2));
-
 
 const unique attPid : Pid;
 const unique helperPid : Pid;
@@ -52,17 +52,20 @@ const unique uid02 : Uid;
 
 const unique UNIL0: Uid;
 
-
 axiom ((uid01 != UNIL0) && (uid02 != UNIL0));
 
-
+///////////////////////////////////////////////////////////////////////////////
 function {:builtin "((as const (Array Int Int)) 0)"} I0() returns ([Uid] int);
 function {:builtin "((as const (Array Int Bool)) False)"} I1() returns ([Uid] bool);
+///////////////////////////////////////////////////////////////////////////////
 
-//  Process session	
+////////////////////////////////////////////////////////////////////////////////
+// Procedure of a process
+////////////////////////////////////////////////////////////////////////////////
 	
 procedure {:yields} {:layer 2} process({:linear "pid"} pid:Pid, {:linear "uid"} uid1: Uid, uid2: Uid)
-requires {:layer 2} ((pid == attPid && uid1 == uid01 && uid2 == uid02) || (pid == helperPid && uid1 == uid02 && uid2 == uid01));
+requires {:layer 2} ((pid == attPid && uid1 == uid01 && uid2 == uid02) || 
+                     (pid == helperPid && uid1 == uid02 && uid2 == uid01));
 {
     var tweet     : int;
   
@@ -106,6 +109,10 @@ requires {:layer 2} ((pid == attPid && uid1 == uid01 && uid2 == uid02) || (pid =
     yield;
 }
 
+///////////////////////////////////////////////////////////////////////////////
+/// An init procedure for initializing the auxiliary variables
+///////////////////////////////////////////////////////////////////////////////
+
 procedure  {:atomic} {:layer 2}  init()
 {
   assume !hb;
@@ -119,23 +126,27 @@ ensures {:layer 1} !hb;
 ensures {:layer 1} (varAtt1 == UNIL0 && varAtt2 == UNIL0 && !att);
 ensures {:layer 1} (forall pid:Pid, uid3:Uid, uid4:Uid::  hbd[pid][uid3][uid4] == 0) ;
 
+///////////////////////////////////////////////////////////////////////////////
+/// The instrumented Twitter transactions
+///////////////////////////////////////////////////////////////////////////////
 
-procedure {:atomic}{:layer 2}  addUser(uid:Uid, p: int)
-modifies ActiveUser, UserPassword;
+procedure {:atomic}{:layer 2}  register(uid:Uid, p: int)
+modifies RegistredUsers, UserPassword;
 {  
-    assume (!ActiveUser[uid] &&  p != 0);
+    assume (!RegistredUsers[uid] &&  p != 0);
  
-    ActiveUser[uid] := true; 
+    RegistredUsers[uid] := true; 
     UserPassword[uid] := p;  
 }
-procedure{:yields}{:layer 1} {:refines "addUser"} AddUser(uid:Uid, p: int);
+procedure{:yields}{:layer 1} {:refines "register"} Register(uid:Uid, p: int);
 
+///////////////////////////////////////////////////////////////////////////////
 
 procedure {:atomic}{:layer 2}  fellowUser(pid:Pid, {:linear "uid"} uid1:Uid, uid2:Uid)
 modifies UserFollow, copyUserFollow;
 modifies hb, hbd, att, varAtt1, varAtt2;
 {  
-    assume (!UserFollow[uid1][uid2] && ActiveUser[uid1] && ActiveUser[uid2] && uid1 != uid2);
+    assume (!UserFollow[uid1][uid2] && RegistredUsers[uid1] && RegistredUsers[uid2] && uid1 != uid2);
 
     if (pid == attPid && !att)
 	{ 
@@ -164,6 +175,8 @@ modifies hb, hbd, att, varAtt1, varAtt2;
 }
 procedure{:yields}{:layer 1} {:refines "fellowUser"} FellowUser(pid:Pid, {:linear "uid"} uid1:Uid, uid2:Uid);
 
+///////////////////////////////////////////////////////////////////////////////
+
 procedure {:atomic}{:layer 2}  addTweet(pid:Pid, {:linear "uid"} uid:Uid, tweet: int)
 modifies UserTweetFollowers, copyUserTweetFollowers;
 modifies hbd;
@@ -172,7 +185,7 @@ modifies hbd;
     var hbd1 : [Uid][Uid]int;
     var hbd2 : [Uid][Uid]int;
 
-    assume (ActiveUser[uid] && tweet != 0);
+    assume (RegistredUsers[uid] && tweet != 0);
 
     if (pid == attPid && att)
 	{ 
