examples/Twitter/Twitter-Original.bpl
@@ -1,56 +1,61 @@
 // Twitter Application
+// It has 3 transactions: register, fellowUser, and addTweet
 
 type Pid;
 type Uid;
 
 function {:builtin "MapConst"} MapConstBool(bool) : [Pid]bool;
-function {:inline} {:linear "pid"} TidCollector(x: Pid) : [Pid]bool
+function {:inline} {:linear "pid"} PidCollector(x: Pid) : [Pid]bool
 {
   MapConstBool(false)[x := true]
 }
 
 function {:builtin "MapConst"} MapConstBool2(bool) : [Uid]bool;
-function {:inline} {:linear "uid"} TidCollector2(x: Uid) : [Uid]bool
+function {:inline} {:linear "uid"} UidCollector(x: Uid) : [Uid]bool
 {
   MapConstBool2(false)[x := true]
 }
 
-var {:layer 0,2} ActiveUser: [Uid]bool;
+var {:layer 0,2} RegistredUsers: [Uid]bool;
 var {:layer 0,2} UserPassword: [Uid]int;
 var {:layer 0,2} UserFollow: [Uid][Uid]bool;
 var {:layer 0,2} UserTweetFollowers: [Uid][Uid]int;
 
+///////////////////////////////////////////////////////////////////////////////
+/// Twitter transactions
+///////////////////////////////////////////////////////////////////////////////
 
-
-procedure {:atomic}{:layer 2}  addUser(uid:Uid, p: int)
-modifies ActiveUser, UserPassword;
+procedure {:atomic}{:layer 2}  register(uid:Uid, p: int)
+modifies RegistredUsers, UserPassword;
 {  
-    assume (!ActiveUser[uid] && p != 0);
+    assume (!RegistredUsers[uid] && p != 0);
     
-	ActiveUser[uid] := true; 
+	RegistredUsers[uid] := true; 
     UserPassword[uid] := p;
 }
-procedure{:yields}{:layer 1} {:refines "addUser"} AddUser(uid:Uid, p: int);
-ensures {:layer 1} ( (!old(ActiveUser[uid]) && p != 0) ==> (ActiveUser[uid] && UserPassword[uid] == p) );
+procedure{:yields}{:layer 1} {:refines "register"} Register(uid:Uid, p: int);
+ensures {:layer 1} ( (!old(RegistredUsers[uid]) && p != 0) ==> (RegistredUsers[uid] && UserPassword[uid] == p) );
 
+///////////////////////////////////////////////////////////////////////////////
 
 procedure {:atomic}{:layer 2}  fellowUser({:linear "uid"} uid1:Uid, uid2:Uid)
 modifies UserFollow;
 {  
-    assume (!UserFollow[uid1][uid2] && ActiveUser[uid1] && ActiveUser[uid2] && uid1 != uid2);
+    assume (!UserFollow[uid1][uid2] && RegistredUsers[uid1] && RegistredUsers[uid2] && uid1 != uid2);
     
 	UserFollow[uid1][uid2] := true; 
 }
 procedure{:yields}{:layer 1} {:refines "fellowUser"} FellowUser({:linear "uid"} uid1:Uid, uid2:Uid);
-ensures {:layer 1} ( (!old(UserFollow[uid1][uid2]) && ActiveUser[uid1] && ActiveUser[uid2] && uid1 != uid2) ==> UserFollow[uid1][uid2] );
+ensures {:layer 1} ( (!old(UserFollow[uid1][uid2]) && RegistredUsers[uid1] && RegistredUsers[uid2] && uid1 != uid2) ==> UserFollow[uid1][uid2] );
 
+///////////////////////////////////////////////////////////////////////////////
 
 procedure {:atomic}{:layer 2}  addTweet({:linear "uid"} uid:Uid, tweet: int)
 modifies UserTweetFollowers;
 {  
     var copyTweet1, copyTweet2 : [Uid]int;	
 
-    assume (ActiveUser[uid] && tweet != 0);
+    assume (RegistredUsers[uid] && tweet != 0);
       
     copyTweet1 := UserTweetFollowers[uid];
 	UserTweetFollowers[uid]  := copyTweet2;
@@ -60,6 +65,6 @@ modifies UserTweetFollowers;
     assume(forall uid0:Uid :: !UserFollow[uid0][uid] ==> (UserTweetFollowers[uid][uid0] == copyTweet1[uid0])); 
 }
 procedure{:yields}{:layer 1} {:refines "addTweet"} AddTweet({:linear "uid"} uid:Uid, tweet: int);
-ensures {:layer 1} ( (ActiveUser[uid] && tweet != 0) ==> 
-        ( (forall uid0:Uid :: (ActiveUser[uid0] && UserFollow[uid0][uid]) ==> (UserTweetFollowers[uid][uid0] == old(UserTweetFollowers[uid][uid0]) + tweet)) &&
-          (forall uid0:Uid :: (!ActiveUser[uid0] || !UserFollow[uid0][uid]) ==> (UserTweetFollowers[uid][uid0] == old(UserTweetFollowers[uid][uid0]))) ) );
+ensures {:layer 1} ( (RegistredUsers[uid] && tweet != 0) ==> 
+        ( (forall uid0:Uid :: (RegistredUsers[uid0] && UserFollow[uid0][uid]) ==> (UserTweetFollowers[uid][uid0] == old(UserTweetFollowers[uid][uid0]) + tweet)) &&
+          (forall uid0:Uid :: (!RegistredUsers[uid0] || !UserFollow[uid0][uid]) ==> (UserTweetFollowers[uid][uid0] == old(UserTweetFollowers[uid][uid0]))) ) );
